Finish new style lists

src/lists.lean
@@ -2,80 +2,71 @@ import polyfix
 import polysize
 import data.list.basic
 
-#exit
-section foldl_lemmas
+section foldl
+variables {α γ : Type*}
 
-variables {α β γ : Type*} [inhabited γ]
-open part_eval (with_time eval)
+def tails_foldl_step (f : α → list γ → α) (x : list γ × α) : bool × (list γ × α) :=
+(x.1.empty, x.1.tail, f x.2 x.1)
 
-def foldl_step (f : α → γ → α) (x : list γ × α) : option (list γ × α) :=
-if x.1.empty then none else some (x.1.tail, f x.2 x.1.head)
-
-theorem foldl_step_eval (f : α → γ → α) (x : list γ × α) (t : ℕ) :
-  eval (with_time (foldl_step f : list γ × α →. option (list γ × α)) (pfun.pure 1)) (t, x) =
-  part.some (t + x.1.length, [], x.1.foldl f x.2) :=
+variables (f : α → list γ → α) (x : list γ × α)
+lemma tails_foldl_step_iter :
+  iterator_evaln (tails_foldl_step f) (2 + x.1.length) (ff, x) = some ([], x.1.tails.foldl f x.2) :=
 begin
-  rcases x with ⟨l, acc⟩, rw [part.eq_some_iff, part_eval.mem_eval],
-  split, swap, { simp [with_time, foldl_step, pfun.pure], },
-  induction l with hd tl ih generalizing acc t, { simp, },
-  have : some (t + 1, tl, f acc hd) ∈ with_time (foldl_step f : list γ × α →. option (list γ × α)) (pfun.pure 1) (t, hd :: tl, acc),
-  { simp [with_time, foldl_step, pfun.pure], },
-  refine (part_eval.reaches_fwd this).trans _, simp at ⊢ ih, specialize ih (f acc hd) (t + 1),
-  rw (show (t + (tl.length + 1) = t + 1 + tl.length), by ac_refl), exact ih,
+  cases x with l x,
+  induction l with hd tl ih generalizing x,
+  { simp [tails_foldl_step], }, { simp [tails_foldl_step, ← add_assoc, ih], },
 end
 
-theorem foldl_step_eval' (f : α → γ → α) (x : list γ × α) :
-  ([], x.1.foldl f x.2) ∈ eval (foldl_step f : list γ × α →. option (list γ × α)) x :=
+variables {f}
+lemma tails_foldl_states_suffix {s₀ s : bool × list γ × α} (hs : s ∈ (mk_iterator ↑(tails_foldl_step f) s₀).states) :
+  s.2.1 <:+ s₀.2.1 :=
 begin
-  have : part_eval.frespects (with_time (foldl_step f : list γ × α →. option (list γ × α)) (pfun.pure 1)) (foldl_step f : list γ × α →. option (list γ × α)) _ :=
-  part_eval.with_time_respects (by simp [pfun.pure]),
-  have R := foldl_step_eval f x 0, simp [part.eq_some_iff] at R,
-  exact this.of_eval R,
+  rcases s₀ with ⟨b₀, l₀, s₀⟩,
+  apply execution.step_induction hs; clear hs s,
+  { simp, },
+  rintros ⟨b, l, s⟩ ⟨b', l', s'⟩ _, simp,
+  rintros ih rfl, simp [tails_foldl_step],
+  rintros rfl rfl rfl,
+  exact l.tail_suffix.trans ih,
 end
 
-def foldl_inv (f : α → γ → α) (x₀ : list γ × α) : set (list γ × α) :=
-{s | ∃ i ≤ x₀.1.length, s.1 = x₀.1.drop i ∧ s.2 = (x₀.1.take i).foldl f x₀.2}
+end foldl
 
-theorem foldl_step_invariant (f : α → γ → α) (x₀) ⦃x y : list γ × α⦄ (hx : x ∈ foldl_inv f x₀) (hy : some y = foldl_step f x) :
-  y ∈ foldl_inv f x₀ :=
-begin 
-  rcases x with ⟨x₁, x₂⟩, rcases x₀ with ⟨l₀, acc₀⟩,
-  simp [foldl_inv] at hx ⊢,
-  rcases hx with ⟨i, H, rfl, rfl⟩,
-  by_cases l₀.length ≤ i,
-  { simp [h, foldl_step] at hy, contradiction, },
-  simp [foldl_step, list.empty_iff_eq_nil, list.drop_eq_nil_iff_le, h] at hy,
-  refine ⟨i+1, _, _, _⟩,
-  { rwa [nat.succ_le_iff, lt_iff_not_le], },
-  { rw hy, simp [← list.drop_one], congr' 1, ac_refl, },
-  rw hy, 
-  suffices : l₀.take (i+1) = l₀.take i ++ [(l₀.drop i).head], { simp [this], }, 
-  rw not_le at h,
-  rw [list.drop_eq_nth_le_cons h, list.take_succ, list.nth_le_nth h], simp [option.to_list],
-end
+section
+open ptree.pencodable (encode decode)
+variables {α β γ : Type*} [polycodable α] [polycodable β] [polycodable γ]
+  {f : β → α → list γ → α} {l : β → list γ} (acc : β → α) 
 
-theorem foldl_step_eval_inv (f : α → γ → α) (x : list γ × α) :
-  x.1.length + 1 ∈ part_eval.time_iter (pfun.res (foldl_step f) (foldl_inv f x)) (pfun.pure 1) x :=
+lemma acc_list_polysize_fun_uniform (hl : polysize_fun l) :
+  polysize_fun_uniform (λ (s : β) (y : (mk_iterator ↑(tails_foldl_step (f s)) (ff, l s, acc s)).states), (y : bool × list γ × α).2.1) :=
 begin
-  rw [← pfun.coe_res_inter, ← part_eval.time_iter_invariant],
-  { simp [part_eval.time_iter, pfun.pure, add_comm x.fst.length 1],
-    use [[], x.1.foldl f x.2], rw ← part.eq_some_iff, convert foldl_step_eval f x 0, simp, },
-  { simpa using foldl_step_invariant f x, },
-  use 0, simp,
+  rcases hl with ⟨pi, hpi⟩, use pi, intros s x,
+  refine trans (encode_sizeof_le_of_infix _) (hpi _),
+  exact (tails_foldl_states_suffix (subtype.mem x)).is_infix,
 end
 
-lemma foldl_cons_eq_reverse {δ : Type*} (l : list δ) (xs : list δ) : 
-  list.foldl (λ a b, b :: a) xs l = l.reverse ++ xs :=
-by { induction l with hd tl ih generalizing xs, { simp, }, simp [ih], }
+lemma tails_foldl_polysize_safe (hinit : polysize_fun l)
+  (hf : polysize_fun_safe (λ (s : β × list γ) (x : α), f s.1 x s.2)) :
+  polysize_fun_safe (λ (s : β) (y : (mk_iterator ↑(tails_foldl_step (f s)) (ff, l s, acc s)).states), tails_foldl_step (f s) (y : bool × list γ × α).2) :=
+begin
+  dsimp only [tails_foldl_step] at *,
+  apply polysize_fun_safe.pair_left, { apply polysize_uniform_of_fin_range, },
+  apply polysize_fun_safe.pair_left,
+  { apply polysize_fun_uniform.comp' (polysize_fun_safe.tail _),
+    apply acc_list_polysize_fun_uniform _ hinit, },
+  change polysize_fun_safe (λ x y, (λ (s : β × list γ) (x : α), f s.1 x s.2) (x, (↑y : bool × list γ × α).2.1) (↑y : bool × list γ × α).2.2),
+  apply polysize_fun_safe.comp hf,
+  { apply polysize_fun_uniform.pair, { simpa using polysize_fun.id, }, apply acc_list_polysize_fun_uniform _ hinit, },
+  refine polysize_fun_safe.comp' (polysize_fun_safe.snd _) _, refine polysize_fun_safe.comp' (polysize_fun_safe.snd _) _,
+  use 0, intros, simp [penc_states_encode],
+end
 
-lemma foldr_eq_map {δ ε} (l : list δ) (f : δ → ε) (xs : list ε) : l.foldr (λ a b, f a :: b) xs = (l.map f) ++ xs :=
-by { induction l, { simp, }, simpa, }
-
-end foldl_lemmas
+end
 
 section list
+
 variables {α β γ : Type*} [polycodable α] [polycodable β] [polycodable γ]
-open polycodable (encode decode)
+open ptree.pencodable (encode decode)
 
 variable (H_enc : polytime_fun (λ l : ptree, ptree.equiv_list.symm $ l.equiv_list.map (encode ∘ (@decode γ _))))
 
@@ -85,227 +76,121 @@ local attribute [instance] inh
 include H_enc
 -- List encoding aux; used very frequently, so better have a short name
 def lea : polycodable (list γ) :=
-{ encode := λ l, ptree.equiv_list.symm (l.map encode),
-  decode := λ v, v.equiv_list.map decode,
-  decode_encode := λ _, by simp,
-  polytime_decode := by { rw polytime_fun_iff', simpa using H_enc, } }
+{ polytime_decode := by simpa [encode, decode] using H_enc }
 
-lemma lea_encode (x : list γ) : by haveI := lea H_enc; exact encode x = ptree.equiv_list.symm (x.map encode) := rfl
-lemma lea_decode (x : ptree) : by haveI := lea H_enc; exact (decode x : list γ) = x.equiv_list.map decode := rfl
+lemma polytime_fun.head_aux : polytime_fun (@list.head γ _) :=
+by { letI := lea H_enc, rw polytime_fun_iff', use [code.left, polytime_left], intro x, cases x, { simp, refl, }, simp [ptree.pencodable.encode_list_def], }
 
-
-open part_eval (with_time eval)
-
-lemma polytime_fun.head_aux : by haveI := lea H_enc; exact polytime_fun (@list.head γ _) :=
-by { rw polytime_fun_iff'', use [code.left, polytime_left], intro x, cases x; simp [lea_encode], refl, }
-
-lemma polytime_fun.tail_aux : by haveI := lea H_enc; exact polytime_fun (@list.tail γ) :=
+lemma polytime_fun.tail_aux : polytime_fun (@list.tail γ) :=
 ⟨code.right, polytime_right,
-by { intro x, cases x; simp [lea_decode, lea_encode], }⟩
+by { intro x, cases x; simp [encode, decode], }⟩
 
-lemma polytime_fun.cons_aux : by haveI := lea H_enc; exact polytime_fun₂ (@list.cons γ) :=
+lemma polytime_fun.cons_aux : polytime_fun₂ (@list.cons γ) :=
 ⟨code.id, polytime_id,
-by { intro x, dunfold polycodable.encode, cases x; simp [lea_encode], }⟩
+by { intro x, cases x; simp [encode], }⟩
 
-lemma polytime_fun.is_empty_aux : by haveI := lea H_enc; exact polytime_fun (@list.empty γ) :=
+lemma polytime_fun.is_empty_aux : polytime_fun (@list.empty γ) :=
 by { letI := lea H_enc, classical, convert_to polytime_fun (λ l : list γ, (l = [] : bool)), { ext x, cases x; simp, }, polyfun, }
 
-lemma polytime_fun.foldl_step {f : β → α → γ → α} (hf : polytime_fun₃ f) :
-  (by haveI := lea H_enc; exact (polytime_fun₂ (λ d, foldl_step (f d)))) :=
+lemma polytime_fun.foldl_tails_aux {f : β → α → list γ → α} {l : β → list γ} {acc : β → α}
+  (hf : polytime_fun₃ f) (hl : polytime_fun l) (hacc : polytime_fun acc)
+  (hs : polysize_fun_safe (λ (a : β × list γ) (b : α), f a.1 b a.2)) :
+  polytime_fun (λ s, (l s).tails.foldl (f s) (acc s)) :=
 begin
   letI := lea H_enc,
-  have := polytime_fun.head_aux H_enc, have := polytime_fun.tail_aux H_enc, have := polytime_fun.is_empty_aux H_enc,
-  delta foldl_step,
-  polyfun,
+  suffices : polytime_fun (λ s, (@list.nil γ, (l s).tails.foldl (f s) (acc s))), { exact polytime_fun.snd.comp this, },
+  apply polytime_fun.evaln_of_polysize (λ (s : β) (x : list γ × α), tails_foldl_step (f s) x) (λ x, (ff, l x, acc x)) (λ s, 2 + (l s).length),
+  { dunfold tails_foldl_step, have := polytime_fun.tail_aux H_enc, have := polytime_fun.is_empty_aux H_enc, polyfun, },
+  { polyfun, }, rotate 1,
+  { obtain ⟨q, hq⟩ := polysize_of_polytime_fun hl, use 2 + q, intros s, simpa using (len_le_encode_sizeof _).trans (hq _), },
+  { intro s, simpa using tails_foldl_step_iter (f s) (l s, acc s), },
+  exact tails_foldl_polysize_safe _ (polysize_of_polytime_fun hl) hs,
 end
 
-section encode_sizeof
-
-@[simp] lemma encode_sizeof_nil : by haveI := lea H_enc; exact (encode ([] : list γ)).sizeof = 1 :=
-by simp [lea_encode]
-@[simp] lemma encode_sizeof_cons (a : γ) (b : list γ) :
-  by haveI := lea H_enc; exact (encode (a :: b)).sizeof = 1 + (encode a).sizeof + (encode b).sizeof :=
-by simp [lea_encode]
-
-lemma encode_sizeof_le_of_mem {l : list γ} {x : γ} (hx : x ∈ l) :
-  by haveI := lea H_enc; exact (encode x).sizeof ≤ (encode l).sizeof :=
-begin
-  induction l with hd tl ih, { simp at hx, contradiction, },
-  rcases ((list.mem_cons_iff _ _ _).mp hx) with rfl|h; simp,
-  { linarith only, },
-  linarith only [ih h],
-end
-
-@[simp] lemma encode_sizeof_append (a b : list γ) : by haveI := lea H_enc; exact
-  ((encode (a ++ b)).sizeof : ℤ) = ((encode a).sizeof : ℤ) + (encode b).sizeof - 1 :=
-by { induction a with hd tl ih, { simp, }, simp [ih], ring, }
-
-lemma encode_sizeof_le_of_sublist {a b : list γ} (h : a <+ b) : by haveI := lea H_enc; exact
-  (encode a).sizeof ≤ (encode b).sizeof :=
-begin
-  induction h, { simp, },
-  case list.sublist.cons : l₁ l₂ s₁ H ih { refine ih.trans _, simp, },
-  case list.sublist.cons2 : l₁ l₂ s₁ H ih { simpa, },
-end
-
-lemma encode_sizeof_le_of_infix {a b : list γ} (h : a <:+: b) : by haveI := lea H_enc; exact
-  (encode a).sizeof ≤ (encode b).sizeof :=
-encode_sizeof_le_of_sublist H_enc h.sublist
-
-lemma encode_list_sizeof (l : list γ) : by haveI := lea H_enc; exact 
-  (encode l).sizeof = (l.map (λ x, (encode x).sizeof)).sum + l.length + 1 :=
-by { induction l with hd tl ih, { simp, }, simp [ih], ac_refl, }
-
-@[simp] lemma encode_sizeof_reverse (l : list γ) : by haveI := lea H_enc; exact
-  (encode l.reverse).sizeof = (encode l).sizeof :=
-by { simp [encode_list_sizeof, list.sum_reverse], }
-
-lemma len_le_encode_sizeof (a : list γ) : by haveI := lea H_enc; exact
-  a.length + 1 ≤ (encode a).sizeof :=
-by { induction a with hd tl ih, { simp, }, simp, linarith, }
-
-lemma polysize_fun_map_polysize {f : β → γ → γ} (hf : polysize_fun₂ f) : by haveI := lea H_enc; exact
-  polysize_fun₂ (λ (s : β) (l : list γ), l.map (f s)) :=
-begin
-  letI := lea H_enc,
-  rcases hf with ⟨p, hp⟩,
-  use (polynomial.monomial 1 1) * p + (polynomial.monomial 1 1) + 1, rintro ⟨s, l⟩, dsimp only,
-  conv_lhs { rw encode_list_sizeof, },
-  simp, mono,
-  { refine (list.sum_le_card_nsmul (l.map (λ x, (encode (f s x)).sizeof)) (p.eval $ (encode s).sizeof + (encode l).sizeof + 1) _).trans _, 
-    { intros x hx, simp at hx, rcases hx with ⟨x, hx, rfl⟩, refine (hp ⟨s, x⟩).trans _,
-      apply monotone_polynomial_nat, simpa using encode_sizeof_le_of_mem H_enc hx, },
-    simp, apply mul_le_mul_right', refine (nat.le_succ _).trans ((len_le_encode_sizeof H_enc l).trans _), linarith only, },
-  refine (nat.le_succ _).trans ((len_le_encode_sizeof H_enc l).trans _), linarith only,
-end
-
-end encode_sizeof
-
-theorem polytime_fun.foldl_aux {f : β → α → γ → α} {l : β → list γ} {acc : β → α} 
-  (hf : polytime_fun₃ f) (hl : by haveI := lea H_enc; exact polytime_fun l) (hacc : polytime_fun acc) 
-  (hs : by haveI := lea H_enc; exact polysize_fun₃ (λ (s : β) (x : α) (l : list γ), l.foldl (f s) x)) :
+lemma polytime_fun.foldl_aux {f : β → α → γ → α} {l : β → list γ} {acc : β → α}
+  (hf : polytime_fun₃ f) (hl : polytime_fun l) (hacc : polytime_fun acc)
+  (hs : polysize_fun_safe (λ (a : β × γ) (b : α), f a.1 b a.2)) :
   polytime_fun (λ s, (l s).foldl (f s) (acc s)) :=
 begin
   letI := lea H_enc,
-  suffices : polytime_fun₃ (λ s (L : list γ) (a : α), (@list.nil γ, L.foldl (f s) a)),
-  { have pf : polytime_fun (λ s, (s, l s, acc s)) := by polyfun,
-    exact polytime_fun.comp polytime_fun.snd (polytime_fun.comp this pf), },
-  cases hs with ps hps,
-  refine polytime_fun.eval (λ s : β, foldl_step (f s)) (λ (s : β) (x : list γ × α), ([], x.1.foldl (f s) x.2))
-    _ (polynomial.monomial 1 1) (ps + polynomial.monomial 1 1) _ _,
-  { exact polytime_fun.foldl_step H_enc hf, },
-  { rintros s ⟨l₀, a₀⟩, simp, apply foldl_step_eval', },
-  rintros S ⟨l₀, a₀⟩, use l₀.length + 1, split,
-  { simp, linarith only [len_le_encode_sizeof H_enc l₀], },
-  apply part_eval.time_iter_mono _ (foldl_step_eval_inv (f S) (l₀, a₀)),
-  rintros ⟨l₁, a₁⟩ y, simp [pfun.mem_res], rintros h₁ h₂, refine ⟨_, h₂⟩,
-  simp [foldl_inv] at h₁, rcases h₁ with ⟨i, hi, rfl, rfl⟩,
-  ring_nf, simp, mono,
-  { apply encode_sizeof_le_of_infix, exact (l₀.drop_suffix i).is_infix, },
-  apply le_add_left, simp,
-  specialize hps ⟨S, a₀, l₀.take i⟩, simp at hps, refine hps.trans (monotone_polynomial_nat _ _),
-  ring_nf, simp, exact encode_sizeof_le_of_infix H_enc (l₀.take_prefix i).is_infix,
+  convert_to polytime_fun (λ s, (l s).tails.foldl (λ (a : α) (ls : list γ), if ls.empty then a else f s a ls.head) (acc s)),
+  { ext s, generalize : acc s = a, induction l s with hd tl ih generalizing a, { simp, }, simp [ih], },
+  apply polytime_fun.foldl_tails_aux H_enc,
+  { have := polytime_fun.head_aux H_enc, have := polytime_fun.is_empty_aux H_enc, polyfun, },
+  { exact hl, }, { exact hacc, },
+  apply polysize_fun_safe.ite, { apply polysize_fun_safe.id, }, 
+  change polysize_fun_safe (λ (x : β × list γ) (y : α), (λ (a : β × γ) (b : α), f a.1 b a.2) (x.1, x.2.head) y),
+  apply hs.comp, { have := polytime_fun.head_aux H_enc, simp, apply polysize_of_polytime_fun, polyfun, }, { exact polysize_fun_safe.id, },
 end
 
-theorem polytime_fun.reverse_aux : by haveI := lea H_enc; exact
-  polytime_fun (@list.reverse γ) :=
+lemma polytime_fun.reverse_aux : polytime_fun (@list.reverse γ) :=
 begin
   letI := lea H_enc,
   convert_to polytime_fun (λ l : list γ, l.foldl (λ acc hd, hd :: acc) []),
-  { ext l : 1, simp [foldl_cons_eq_reverse], },
-  apply polytime_fun.foldl_aux,
-  { have := polytime_fun.cons_aux H_enc, polyfun, },
-  { exact polytime_fun.id, }, { exact polytime_fun.const _, },
-  simp [foldl_cons_eq_reverse], use polynomial.monomial 1 1,
-  rintro ⟨a, b, c⟩, zify, simp, linarith only,
+  { ext l : 1, rw ← list.foldr_reverse, simp, },
+  apply polytime_fun.foldl_aux H_enc, { have := polytime_fun.cons_aux H_enc, polyfun, }, { polyfun, }, { polyfun, },
+  apply polysize_fun_safe.comp polysize_fun_safe.cons, { simp, apply polysize_of_polytime_fun, polyfun, }, exact polysize_fun_safe.id,
 end
 
-theorem polytime_fun.foldr_aux {f : β → γ → α → α} {l : β → list γ} {acc : β → α} 
-  (hf : polytime_fun₃ f) (hl : by haveI := lea H_enc; exact polytime_fun l) (hacc : polytime_fun acc) 
-  (hs : by haveI := lea H_enc; exact polysize_fun₃ (λ (s : β) (x : α) (l : list γ), l.foldr (f s) x)) :
+lemma polytime_fun.foldr_aux {f : β → γ → α → α} {l : β → list γ} {acc : β → α}
+  (hf : polytime_fun₃ f) (hl : polytime_fun l) (hacc : polytime_fun acc)
+  (hs : polysize_fun_safe (λ (a : β × γ) (b : α), f a.1 a.2 b)) :
   polytime_fun (λ s, (l s).foldr (f s) (acc s)) :=
 begin
   letI := lea H_enc,
-  simp only [← list.foldl_reverse], apply polytime_fun.foldl_aux,
-  { polyfun, },
-  { apply polytime_fun.comp (polytime_fun.reverse_aux H_enc) hl, },
-  { exact hacc, },
-  simp only [← list.foldr_reverse],
-  suffices : polysize_fun (λ xls : β × α × list γ, (xls.1, xls.2.1, xls.2.2.reverse)),
-  { exact polysize_fun.comp hs this, },
-  apply polysize_of_polytime_fun,
-  have := polytime_fun.reverse_aux H_enc, polyfun,
+  simp only [← list.foldl_reverse],
+  apply polytime_fun.foldl_aux H_enc, { polyfun, }, { have := polytime_fun.reverse_aux H_enc, polyfun, }, { polyfun, },
+  exact hs,
 end
 
-lemma polysize_fun.append : by haveI := lea H_enc; exact
-  polysize_fun₂ (@list.append γ) :=
-⟨polynomial.monomial 1 1,
-by { rintro ⟨a, b⟩, zify, simp [list.append_eq_has_append], linarith, }⟩
-
-theorem polytime_fun.map_aux {f : β → γ → γ} {l : β → list γ}
-  (hf : polytime_fun₂ f)
-  (hl : by haveI := lea H_enc; exact polytime_fun l) : by haveI := lea H_enc; exact
+lemma polytime_fun.map_aux 
+  (H_enc' : polytime_fun (λ l : ptree, ptree.equiv_list.symm $ l.equiv_list.map (encode ∘ (@decode α _))))
+  {f : β → γ → α} {l : β → list γ} (hf : polytime_fun₂ f) (hl : polytime_fun l) :
   polytime_fun (λ s, (l s).map (f s)) :=
 begin
-  letI := lea H_enc,
-  convert_to polytime_fun (λ s : β, (l s).foldr (λ a b, f s a :: b) []),
-  { ext s : 1, simp [foldr_eq_map], },
-  apply polytime_fun.foldr_aux,
-  { have := polytime_fun.cons_aux H_enc, polyfun, },
-  { exact hl, }, { apply polytime_fun.const, },
-  simp only [foldr_eq_map],
-  apply polysize_fun.comp₂ (polysize_fun.append H_enc),
-  { refine polysize_fun.comp (polysize_fun_map_polysize H_enc (polysize₂_of_polytime₂ hf)) (_ : polysize_fun (λ s : β × list γ × list γ, (s.1, s.2.2))), 
-    apply polysize_of_polytime_fun, polyfun, },
-  apply polysize_of_polytime_fun, polyfun,
+  letI := lea H_enc, letI := lea H_enc',
+  convert_to polytime_fun (λ s, (l s).foldr (λ hd acc, (f s hd) :: acc) []),
+  { ext s : 1, induction l s with hd tl ih, { simp, }, simp [ih], },
+  apply polytime_fun.foldr_aux H_enc,
+  { have := polytime_fun.cons_aux H_enc', polyfun, }, { exact hl, }, { polyfun, },
+  apply polysize_fun_safe.comp polysize_fun_safe.cons, { simp, apply polysize_of_polytime_fun, exact hf, }, { exact polysize_fun_safe.id, },
 end
 
 end list
 
+
 section list_ptree
-open polycodable (encode decode)
+open ptree.pencodable (encode decode)
 
 def list_ptree_encode : polycodable (list ptree) :=
 lea ⟨code.id, polytime_id, by simp [encode, decode]⟩
 
 local attribute [instance] list_ptree_encode
 
+@[polyfun]
+lemma polytime_fun.equiv_list : polytime_fun ptree.equiv_list :=
+⟨_, polytime_id, by simp [encode]⟩
+
+@[polyfun]
+lemma polytime_fun.equiv_list_symm : polytime_fun ptree.equiv_list.symm :=
+⟨_, polytime_id, by simp [encode]⟩
+
 lemma H_enc {γ : Type*} [polycodable γ] : 
   polytime_fun (λ l : ptree, ptree.equiv_list.symm $ l.equiv_list.map (encode ∘ (@decode γ _))) :=
 begin
-  suffices : polytime_fun (λ l : list ptree, l.map (encode ∘ (@decode γ _))),
-  { rcases this with ⟨c, pc, s⟩, use [c, pc], intro x, specialize s x.equiv_list, simp [encode, list_ptree_encode, lea_encode] at s, simp [s], },
-  apply polytime_fun.map_aux; polyfun,
+  refine polytime_fun.equiv_list_symm.comp (polytime_fun.comp _ polytime_fun.equiv_list),
+  apply polytime_fun.map_aux, iterate 2 { simpa using polytime_fun.id, },
+  { /- TODO: Debug -/ dunfold polytime_fun₂ function.uncurry, apply polytime_fun.comp; polyfun, }, polyfun,
 end
 
 end list_ptree
 
 section list
-open polycodable (encode decode)
+open ptree.pencodable (encode decode)
 
 variables {α β γ : Type*} [polycodable α] [polycodable β] [polycodable γ]
 instance : polycodable (list α) :=
 lea H_enc
-
-@[higher_order]
-lemma polycodable.list_encode (l : list α) :
-  encode l = ptree.equiv_list.symm (l.map encode) := rfl
-@[higher_order]
-lemma polycodable.list_decode (v : ptree) :
-  @decode (list α) _ v = (ptree.equiv_list v).map decode := rfl
-@[simp] lemma polycodable.list_ptree_encode :
-  @encode (list ptree) _ = ptree.equiv_list.symm :=
-by { ext l, rw polycodable.list_encode, simp, erw l.map_id, }
-@[simp] lemma polycodable.list_ptree_decode :
-  @decode (list ptree) _ = ptree.equiv_list :=
-by { ext l, rw polycodable.list_decode, erw l.equiv_list.map_id, }
-
-@[polyfun]
-lemma polytime_fun.ptree_equiv_list : polytime_fun ptree.equiv_list :=
-by { rw ← polycodable.list_ptree_decode, polyfun, }
-@[polyfun]
-lemma polytime_fun.ptree_equiv_list_symm : polytime_fun ptree.equiv_list.symm :=
-by { rw ← polycodable.list_ptree_encode, polyfun, }
 
 
 lemma polytime_fun.head : polytime_fun (@list.head γ ⟨decode ptree.nil⟩) :=
@@ -341,121 +226,56 @@ end
 
 local attribute [-polyfun] polytime_fun.head
 
-@[polyfun]
-theorem polytime_fun.foldr {f : β → γ → α → α} {l : β → list γ} {acc : β → α} 
-  (hf : polytime_fun₃ f) (hl : polytime_fun l) (hacc : polytime_fun acc) 
-  (hs : polysize_fun₃ (λ (s : β) (x : α) (l : list γ), l.foldr (f s) x)) :
-  polytime_fun (λ s, (l s).foldr (f s) (acc s)) :=
-polytime_fun.foldr_aux H_enc hf hl hacc hs
+lemma polytime_fun.foldl_tails {f : β → α → list γ → α} {l : β → list γ} {acc : β → α}
+  (hf : polytime_fun₃ f) (hl : polytime_fun l) (hacc : polytime_fun acc)
+  (hs : polysize_fun_safe (λ (a : β × list γ) (b : α), f a.1 b a.2)) :
+  polytime_fun (λ s, (l s).tails.foldl (f s) (acc s)) := polytime_fun.foldl_tails_aux H_enc hf hl hacc hs
 
 @[polyfun]
-theorem polytime_fun.reverse : polytime_fun (@list.reverse γ) :=
-polytime_fun.reverse_aux H_enc
+lemma polytime_fun.foldl {f : β → α → γ → α} {l : β → list γ} {acc : β → α}
+  (hf : polytime_fun₃ f) (hl : polytime_fun l) (hacc : polytime_fun acc)
+  (hs : polysize_fun_safe (λ (a : β × γ) (b : α), f a.1 b a.2)) :
+  polytime_fun (λ s, (l s).foldl (f s) (acc s)) := polytime_fun.foldl_aux H_enc hf hl hacc hs
 
 @[polyfun]
-theorem polytime_fun.foldl {f : β → α → γ → α} {l : β → list γ} {acc : β → α} 
-  (hf : polytime_fun₃ f) (hl : polytime_fun l) (hacc : polytime_fun acc) 
-  (hs : polysize_fun₃ (λ (s : β) (x : α) (l : list γ), l.foldl (f s) x)) :
-  polytime_fun (λ s, (l s).foldl (f s) (acc s)) :=
-polytime_fun.foldl_aux H_enc hf hl hacc hs
+lemma polytime_fun.reverse : polytime_fun (@list.reverse γ) := polytime_fun.reverse_aux H_enc
 
 @[polyfun]
-theorem polytime_fun.map {f : β → γ → α} {l : β → list γ}
-  (hf : polytime_fun₂ f)
-  (hl : polytime_fun l) :
-  polytime_fun (λ s, (l s).map (f s)) :=
+lemma polytime_fun.foldr {f : β → γ → α → α} {l : β → list γ} {acc : β → α}
+  (hf : polytime_fun₃ f) (hl : polytime_fun l) (hacc : polytime_fun acc)
+  (hs : polysize_fun_safe (λ (a : β × γ) (b : α), f a.1 a.2 b)) :
+  polytime_fun (λ s, (l s).foldr (f s) (acc s)) := polytime_fun.foldr_aux H_enc hf hl hacc hs
+
+@[polyfun]
+lemma polytime_fun.map 
+  {f : β → γ → α} {l : β → list γ} (hf : polytime_fun₂ f) (hl : polytime_fun l) :
+  polytime_fun (λ s, (l s).map (f s)) := polytime_fun.map_aux H_enc H_enc hf hl
+
+@[polyfun]
+lemma polytime_fun.filter {f : β → γ → bool} {l : β → list γ} (hf : polytime_fun₂ f) (hl : polytime_fun l) :
+  polytime_fun (λ s, (l s).filter (λ x, f s x)) :=
 begin
-  have H₁ : polytime_fun (λ l : list γ, l.map encode),
-  { apply polytime_fun.decode, simp, apply polytime_fun.encode, },
-  have H₂ : polytime_fun (λ (S : β × list ptree), S.2.map (encode ∘ (f S.1) ∘ decode)),
-  { apply polytime_fun.map_aux H_enc; polyfun, },
-  have H₃ : polytime_fun (λ l : list ptree, l.map (@decode α _)),
-  { apply polytime_fun.decode, simp [polycodable.list_encode'],
-    apply polytime_fun.comp polytime_fun.ptree_equiv_list_symm, simp, apply polytime_fun.map_aux H_enc; polyfun, },
-  have H₁' : polytime_fun (λ (s : β), (s, (l s).map encode)), { polyfun, },
-  convert H₃.comp (H₂.comp H₁'), ext, simp,
-end
-
-lemma foldr_eta' (l₁ l₂ : list α) : l₁.foldr list.cons l₂ = l₁ ++ l₂ :=
-by { induction l₁ with hd tl ih, { simp, }, simpa, }
-
-lemma len_le_encode_sizeof' (l : list α) :
-  l.length ≤ (encode l).sizeof :=
-by { refine (nat.le_succ _).trans _, apply len_le_encode_sizeof, }
-
-theorem polysize_foldl (f : β → α → γ → α) (hf : ∃ p : polynomial ℕ, ∀ s acc hd, (encode (f s acc hd)).sizeof ≤ (encode acc).sizeof + p.eval (encode (s, hd)).sizeof) :
-  polysize_fun₃ (λ (s : β) (x : α) (l : list γ), l.foldl (f s) x) :=
-begin
-  rcases hf with ⟨p, hp⟩,
-  have : ∀ (s : β) (x : α) (l : list γ), (encode (l.foldl (f s) x)).sizeof ≤ (encode x).sizeof + (p.eval (encode (s, l)).sizeof) * l.length,
-  { intros s x l, induction l with hd tl ih generalizing x, { simp, },
-    simp, refine (ih _).trans _, rw [add_comm tl.length 1, mul_add, ← add_assoc], 
-    mono*, { refine (hp _ _ _).trans _, simp, apply monotone_polynomial_nat, linarith only, },
-    all_goals { simp, }, }, 
-  use polynomial.monomial 1 1 + p * (polynomial.monomial 1 1),
-  rintros ⟨s, x, l⟩, simp, refine (this _ _ _).trans _, mono*,
-  { linarith only, }, { simp, linarith only, },
-  refine (len_le_encode_sizeof' _).trans _, all_goals { linarith only, },
-end
-
-theorem polysize_foldr {f : β → γ → α → α} (hf : ∃ p : polynomial ℕ, ∀ s hd acc, (encode (f s hd acc)).sizeof ≤ (encode acc).sizeof + p.eval (encode (s, hd)).sizeof) :
-  polysize_fun₃ (λ (s : β) (x : α) (l : list γ), l.foldr (f s) x) :=
-begin
-  simp_rw ← list.foldl_reverse, dunfold polysize_fun₃,
-  refine polysize_fun.comp (_ : polysize_fun (λ sxl : β × α × list γ, sxl.2.2.foldl (λ y x, f sxl.1 x y) sxl.2.1)) (_ : polysize_fun (λ sxl : β × α × list γ, (sxl.1, sxl.2.1, sxl.2.2.reverse))),
-  { skip, apply polysize_foldl (λ s acc hd, f s hd acc), dsimp, rcases hf with ⟨p, hp⟩, use p, intros, apply hp, },
-  { apply polysize_of_polytime_fun, polyfun, },
+  convert_to polytime_fun (λ s, (l s).foldr (λ hd acc, if f s hd then hd :: acc else acc) []),
+  { ext s : 1, induction l s with hd tl ih, { simp, }, cases H : f s hd; simpa [H], },
+  polyfun, apply polysize_fun_safe.ite, { refine polysize_fun_safe.comp polysize_fun_safe.cons _ polysize_fun_safe.id, simp, exact polysize_of_polytime_fun polytime_fun.snd, }, exact polysize_fun_safe.id,
 end
 
 @[polyfun]
-theorem polytime_fun.append : polytime_fun₂ (@list.append γ) :=
+lemma polytime_fun.append : polytime_fun₂ (λ (l₁ l₂ : list α), l₁ ++ l₂) :=
 begin
-  change polytime_fun₂ (λ (l₁ l₂ : list γ), l₁ ++ l₂), simp_rw ← foldr_eta', polyfun,
-  use polynomial.monomial 1 1, rintro ⟨⟨a, b⟩, c, d⟩,  simp_rw foldr_eta', zify, simp, linarith only,
+  convert_to polytime_fun₂ (λ (l₁ l₂ : list α), l₁.foldr list.cons l₂),
+  { ext l₁ l₂ : 2, induction l₁ with hd tl ih, { simp, }, { simp [ih], } },
+  polyfun, apply polysize_fun_safe.cons.comp, { simp, apply polysize_of_polytime_fun polytime_fun.snd, }, exact polysize_fun_safe.id,
 end
 
 @[polyfun]
-lemma polytime_fun.append₂ : polytime_fun₂ (λ (a b : list α), a ++ b) := polytime_fun.append
-
-section bool
-
-@[polyfun]
-lemma polytime_fun.all {f : β → α → bool} {l : β → list α} (hf : polytime_fun₂ f) (hl : polytime_fun l) :
-  polytime_fun (λ s, (l s).all (f s)) :=
-by { simp only [list.all], polyfun, apply polysize_fun_of_fin_range, }
-
-@[polyfun]
-lemma polytime_fun.any {f : β → α → bool} {l : β → list α} (hf : polytime_fun₂ f) (hl : polytime_fun l) :
-  polytime_fun (λ s, (l s).any (f s)) :=
-by { simp only [list.any], polyfun, apply polysize_fun_of_fin_range, }
-
-end bool
-
-@[polyfun]
-lemma polytime_fun.last : polytime_fun (@list.last' α) :=
+lemma polytime_fun.tails : polytime_fun (@list.tails α) :=
 begin
-  convert_to polytime_fun (λ l : list α, l.reverse.head'), { ext l : 1, induction l using list.reverse_rec_on; simp, },
-  polyfun,
+  convert_to polytime_fun (λ l : list α, (l.tails.foldl (λ acc x, x :: acc) []).reverse),
+  { simp, }, apply polytime_fun.comp, { polyfun, }, apply polytime_fun.foldl_tails,
+  { polyfun, }, { polyfun, }, { polyfun, }, apply polysize_fun_safe.cons.comp, { simp, apply polysize_of_polytime_fun polytime_fun.snd, }, exact polysize_fun_safe.id,
 end
 
-lemma polytime_fun.filter {f : β → α → bool} {l : β → list α} (hf : polytime_fun₂ f)
-  (hl : polytime_fun l) : polytime_fun (λ s, (l s).filter (λ x, f s x)) :=
-begin
-  have filter_eq : ∀ (xs : list α) (l : list α) (P : α → bool), l.foldr (λ hd acc, if P hd then hd :: acc else acc) xs = (l.filter (λ x, P x)) ++ xs,
-  { intros xs l P, induction l with hd tl ih, { simp, }, cases H : P hd; simpa [H], },
-  convert_to polytime_fun (λ s : β, (l s).foldr (λ hd acc, if f s hd then hd :: acc else acc) []),
-  { ext s : 1, simp [filter_eq], }, polyfun,
-  apply polysize_foldr, 
-  use polynomial.monomial 1 1, 
-  intros s hd acc, split_ifs; simp, linarith only,
-end
-
-@[simp]
-def list.izip {α β : Type*} [inhabited α] [inhabited β] : list α → list β → list (α × β)
-| (x :: xs) (y :: ys) := (x, y) :: (xs.izip ys)
-| [] (y :: ys) := (default, y) :: (list.izip [] ys)
-| (x :: xs) [] := (x, default) :: (list.izip xs [])
-| [] [] := []
 
 def unary_nat_encode : polycodable ℕ := 
 polycodable.of_equiv equiv.list_unit_equiv.symm
@@ -468,7 +288,7 @@ lemma unary_nat_encode_eq (n : ℕ) : encode n = encode (list.repeat () n) := rf
 lemma polytime_fun.unary_length : polytime_fun (@list.length α) :=
 begin
   convert_to polytime_fun (λ l : list α, equiv.list_unit_equiv (l.map (λ _, ()))),
-  { ext l, simp [equiv.list_unit_equiv], }, polyfun,
+  { ext l, simp [equiv.list_unit_equiv], }, polyfun, exact polycodable.of_equiv_polytime_symm _,
 end
 
 @[polyfun]
@@ -485,80 +305,16 @@ begin
   { ext, simp, }, polyfun,
 end
 
-@[simp] lemma encode_unit_sizeof : (encode ()).sizeof = 1 :=
-by { simp [encode], }
-
-@[simp] lemma encode_unary_nat_sizeof (n : ℕ) : (encode n).sizeof = 2 * n + 1 :=
-by { simp [unary_nat_encode_eq, encode_list_sizeof], ring, }
-
-@[polyfun]
-lemma polytime_fun.unary_iterate {f : α → β → β} {n : α → ℕ} (hf : polytime_fun₂ f) (hn : polytime_fun n)
-  (H : polysize_fun₃ (λ s (i : ℕ), (f s)^[i])) : polytime_fun₂ (λ s, (f s)^[n s]) :=
-begin
-  convert_to polytime_fun₂ (λ (s : α) (x : β), (list.repeat () (n s)).foldr (λ _, f s) x),
-  { simp [list.foldr_const], },
-  polyfun, change polysize_fun₃ (λ s x l, _), simp [list.foldr_const],
-  refine H.comp (_ : polysize_fun (λ (sxl : (α × β) × β × list unit), (sxl.1.1, sxl.2.2.length, sxl.2.1))),
-  apply polysize_of_polytime_fun, polyfun,
-end
-
-lemma _root_.nat.le_mul_right (a : ℕ) {b : ℕ} (hb : b ≠ 0) : a ≤ a * b :=
-by { cases b, { contradiction, }, simp [nat.mul_succ], }
-
-
-lemma polysize_fun.iterate_of_bounded_growth' {f : α → β → β} (hf : ∃ C : polynomial ℕ, ∀ a b, (encode $ f a b).sizeof ≤ (encode b).sizeof + C.eval (encode a).sizeof) :
-  polysize_fun₃ (λ s (i : ℕ), (f s)^[i]) :=
-begin
-  rcases hf with ⟨c, hc⟩,
-  have : ∀ a b (i : ℕ), (encode ((f a)^[i] b)).sizeof ≤ (encode b).sizeof + (c.eval (encode a).sizeof) * i,
-  { intros a b i, induction i with i ih, { simp, }, simp [function.iterate_succ', nat.mul_succ], refine (hc _ _).trans _, rw ← add_assoc, simpa, },
-  use polynomial.monomial 1 1 + c * (polynomial.monomial 1 1), rintro ⟨s, i, l⟩, simp, refine (this _ _ _).trans _,
-  mono*; linarith only,
-end
-
-lemma polysize_fun.iterate_of_bounded_growth {f : α → β → β} (hf : ∃ C, ∀ a b, (encode $ f a b).sizeof ≤ (encode b).sizeof + C) :
-  polysize_fun₃ (λ s (i : ℕ), (f s)^[i]) :=
-by { rcases hf with ⟨c, hc⟩, apply polysize_fun.iterate_of_bounded_growth', use c, simpa, }
-
-lemma _root_.list.range_sum (n : ℕ) : 2 * (list.range n).sum =  n * (n - 1) :=
-begin
-  induction n with n ih, { simp, },
-  simp [list.range_succ, mul_add, ih],
-  cases n; simp [nat.succ_eq_add_one], ring,
-end
-
-lemma polysize_unary_range : polysize_fun list.range :=
-begin
-  use (polynomial.monomial 2 1), intro x,
-  simp [encode_list_sizeof],
-  rw list.sum_map_mul_left, simp [list.range_sum], cases x, { simp, },
-  simp [nat.succ_eq_add_one], nlinarith,
-end
-
-@[polyfun]
-lemma polytime_fun.unary_range : polytime_fun list.range :=
-begin
-  have : ∀ (l : list unit) (xs : list ℕ), l.foldr (λ _ (acc : list ℕ), 0 :: acc.map (+1)) xs =
-    (list.range l.length) ++ (xs.map (+l.length)),
-  { intros l xs, induction l with hd tl ih, { simp, }, simp [list.range_succ_eq_map, ih], },
-  convert_to polytime_fun (λ n, (list.repeat () n).foldr (λ _ (acc : list ℕ), 0 :: acc.map (+1)) []),
-  { ext n : 1, simp [this], }, 
-  polyfun, change polysize_fun₃ (λ s l xs, _), simp only [this],
-  apply polysize_fun.comp₂ (polysize_fun.append _), swap, { apply polysize_of_polytime_fun, polyfun, },
-  apply polysize_fun.comp polysize_unary_range, apply polysize_of_polytime_fun, polyfun,
-end
-
-@[simp] lemma _root_.list.drop_succ {α : Type*} (l : list α) (n : ℕ) :
+lemma _root_.list.drop_succ {α : Type*} (l : list α) (n : ℕ) :
   l.drop (n+1) = l.tail.drop n :=
 by { induction l; simp, }
 
 @[polyfun]
 lemma polytime_fun.drop : polytime_fun₂ (@list.drop α) :=
 begin
-  convert_to polytime_fun₂ (λ n l, list.tail^[n] l),
-  { ext n l : 2, induction n generalizing l; simp [*], },
-  polyfun, apply polysize_fun.iterate_of_bounded_growth, use 0, intros _ b,
-  cases b; simp,
+  convert_to polytime_fun₂ (λ (n : ℕ) (l : list α), (list.repeat () n).foldr (λ _ (l' : list α), l'.tail) l),
+  { ext n l : 2, rw list.foldr_const, simp, induction n generalizing l; simp [list.drop_succ, *], },
+  polyfun, exact polysize_fun_safe.tail _,
 end
 
 @[polyfun]
@@ -570,102 +326,57 @@ begin
 end
 
 @[polyfun]
-lemma polytime_fun.inth [inhabited α] : polytime_fun₂ (@list.inth α _) :=
-by { change polytime_fun₂ (λ (l : list α) n, (l.nth n).iget), polyfun, }
-
-@[polyfun]
-lemma polytime_fun.unary_nat_tsub : polytime_fun₂ (has_sub.sub : ℕ → ℕ → ℕ) :=
+lemma polytime_fun.tsub : polytime_fun₂ (@has_sub.sub ℕ _) :=
 begin
-  convert_to polytime_fun₂ (λ m n, ((list.repeat () m).drop n).length),
+  convert_to polytime_fun₂ (λ (m n : ℕ), ((list.repeat () m).drop n).length),
   { ext m n, simp, }, polyfun,
 end
 
 @[polyfun]
-lemma polytime_fun.unary_nat_le {f g : α → ℕ} (hf : polytime_fun f) (hg : polytime_fun g) :
-  polytime_fun (λ n, (f n ≤ g n : bool)) :=
+lemma polytime_fun.last : polytime_fun (@list.last' α) :=
+by { convert_to polytime_fun (λ l : list α, l.reverse.head'), { ext l : 1, induction l using list.reverse_rec_on; simp, }, polyfun, }
+
+@[polyfun]
+lemma polytime_fun.filter_map {f : β → α → option γ} {l : β → list α} 
+  (hf : polytime_fun₂ f) (hl : polytime_fun l) :
+  polytime_fun (λ s, (l s).filter_map (f s)) :=
 begin
-  convert_to polytime_fun (λ n, ((f n - g n) = 0 : bool)),
-  { ext n, simp, }, polyfun,
+  inhabit γ,
+  convert_to polytime_fun (λ s, (((l s).map (λ x, f s x)).filter (λ x : option γ, x.is_some)).map option.iget),
+  { ext s : 1, induction l s with hd tl ih, { simp, }, cases H : f s hd, { simpa [H], }, { simpa [list.filter_map_cons_some _ _ _ H, H], } },
+  polyfun,
+end
+
+@[simp] lemma _root_.list.filter_map_none (l : list α) :
+  l.filter_map (λ _, (none : option β)) = [] :=
+by { induction l; simp [*], }
+
+lemma zip_eq_inits_map [inhabited α] (l₁ : list α) (l₂ : list β) :
+  l₁.zip l₂ = l₁.inits.tail.filter_map (λ x, (l₂.nth (x.length - 1)).map (λ y, (x.last'.iget, y))) :=
+begin
+  induction l₁ with hd tl ih generalizing l₂,
+  { simp, },
+  cases l₂ with h₂ t₂, { simp, }, 
+  simp [list.filter_map_map, function.comp], 
+  cases tl, { simp, rw list.filter_map_cons_some, { simp, }, simp, },
+  simp, rw list.filter_map_cons_some, swap, { simp, },
+  rw ih t₂, simp [list.filter_map_map, function.comp],
 end
 
 @[polyfun]
-lemma polytime_fun.unary_nat_min : polytime_fun₂ (@min ℕ _) :=
-by { change polytime_fun₂ (λ n m, if n ≤ m then n else m), polyfun, }
-
-lemma _root_.list.nth_eq_some_nth_le {α} (l : list α) (n : ℕ) (hn : n < l.length) : l.nth n = some (l.nth_le n hn) :=
-by { rw list.nth_eq_some, exact ⟨_, rfl⟩, }
+lemma polytime_fun.inits : polytime_fun (@list.inits α) :=
+by { convert_to polytime_fun (λ l : list α, (l.reverse.tails.map list.reverse).reverse), { simp [list.tails_reverse], }, polyfun, }
 
 @[polyfun]
 lemma polytime_fun.zip : polytime_fun₂ (@list.zip α β) :=
 begin
-  inhabit α, inhabit β,
-  convert_to polytime_fun₂ (λ (l₁ : list α) (l₂ : list β), (list.range $ min l₁.length l₂.length).map (λ i, (l₁.inth i, l₂.inth i))),
-  { ext l₁ l₂ : 2, apply list.ext_le, { simp, }, intros n h₁ h₂, simp [list.inth], rw [list.nth_eq_some_nth_le, list.nth_eq_some_nth_le], exact ⟨rfl, rfl⟩, },
-  polyfun,
-end
-
-@[simp] lemma _root_.list.map_with_index_nil {α β} (f : ℕ → α → β) :
-  (@list.nil α).map_with_index f = [] := rfl
-
-@[simp] lemma _root_.list.map_with_index_snoc {α β} (f : ℕ → α → β) (init : list α) (last : α) :
-  (init ++ [last]).map_with_index f = (init.map_with_index f) ++ [f init.length last] :=
-begin
-  suffices : ∀ n, (init ++ [last]).map_with_index_core f n = (init.map_with_index_core f n) ++ [f (init.length + n) last],
-  { exact this 0, },
-  induction init with hd tl ih,
-  { intro, simp [list.map_with_index_core], },
-  { intro n, simp [list.map_with_index_core, ih (n + 1)], congr' 3, ring, },
-end
-
-theorem _root_.list.map_with_index_eq_zip_map {α β} (l : list α) (f : ℕ → α → β) :
-  l.map_with_index f = (list.zip (list.range l.length) l).map (λ x, f x.1 x.2) :=
-begin
-  induction l using list.reverse_rec_on with int lst ih,
-  { simp, },
-  { simp [list.map_with_index_snoc, ih, list.range_succ],
-    rw list.zip_append; simp, }
+  inhabit α,
+  change polytime_fun₂ (λ l₁ l₂, list.zip l₁ l₂), simp_rw zip_eq_inits_map, polyfun,
 end
 
 @[polyfun]
-lemma polytime_fun.imap {f : α → list β} {g : α → ℕ → β → γ}
-  (hf : polytime_fun f) (hg : polytime_fun₃ g) :
-  polytime_fun (λ s, (f s).map_with_index (g s)) :=
-begin
-  convert_to polytime_fun (λ s, ((list.range $ (f s).length).zip (f s)).map (λ x, g s x.1 x.2)),
-  { ext s : 1, apply list.map_with_index_eq_zip_map, },
-  polyfun,
-end
-
-@[simp]
-def _root_.list.attach_tails {α} : list α → list (list α)
-| [] := []
-| (hd :: tl) := (hd :: tl) :: (_root_.list.attach_tails tl)
-
-@[polyfun]
-lemma polytime_fun.attach_tails : polytime_fun (@list.attach_tails α) :=
-begin
-  convert_to polytime_fun (λ l : list α, l.map_with_index (λ i x, l.drop i)),
-  { ext l : 1, rw list.map_with_index_eq_zip_map, induction l with hd tl ih,
-    { simp, }, simpa [list.range_succ_eq_map,  list.zip_map_left] using ih, },
-  polyfun,
-end
-
-@[simp]
-def _root_.list.rec' {α β} (f : list β → α → α) (s : α) : list β → α
-| [] := s
-| (hd :: tl) := f (hd :: tl) (_root_.list.rec' tl)
-
-@[polyfun]
-lemma polytime_fun.list_rec {f : γ → list β → α → α} {s₀ : γ → α} {l : γ → list β}
-  (hf : polytime_fun₃ f) (hs₀ : polytime_fun s₀) (hl : polytime_fun l) 
-  (hb : ∃ C : polynomial ℕ, ∀ (s : γ) (l : list β) (x : α), (encode $ f s l x).sizeof ≤ (encode x).sizeof + C.eval (encode (s, l)).sizeof) :
-  polytime_fun (λ s, (l s).rec' (f s) (s₀ s)) :=
-begin
-  convert_to polytime_fun (λ s, (l s).attach_tails.foldr (f s) (s₀ s)),
-  { ext s, induction l s, { simp, }, { simp [ih], }, },
-  polyfun,
-  apply polysize_foldr, exact hb,
-end
-
+lemma polytime_fun.all {f : β → α → bool} {l : β → list α} 
+  (hf : polytime_fun₂ f) (hl : polytime_fun l) : polytime_fun (λ s, (l s).all (f s)) :=
+by { dunfold list.all, polyfun, exact (polysize_uniform_of_fin_range _).to_safe, }
 
 end list
